\subsection*{Problem A4} 
    \hfill \break
    Subtract by parts Equations \eqref{eq:16} and \eqref{eq:18}:
    \begin{align}
        \dot{x_1} = x_2 \nonumber\\ 
        \text{--- } \hspace{0.5cm} 0 = x^e \nonumber \\
        \hspace{3cm}\rule{3cm}{1pt} \nonumber \\
        \therefore \dot{\bar{x}} = x_2 - x_2^e \nonumber \\
        = \bar{x_2} \nonumber
    \end{align}
    \hfill \break
    \begin{align}
        \dot{x_2} = \frac{5cI^2}{3m(\delta - x_1)^2} + \frac{5g\sin{\phi}}{3} - \frac{5k}{3m}(x_1 -d) - \frac{5b x_2}{3m}\nonumber\\ 
        \text{--- }  \hspace{2cm}0 = \frac{5cI^e^2}{3m(\delta - x_1^e)^2} + \frac{5g\sin{\phi}}{3} - \frac{5k}{3m}(x_1^e -d)  \nonumber \\
        \rule{10cm}{1pt} \nonumber \\
        \dot{\bar{x_2}} ={\frac{5c}{3m}\left( \frac{I^2}{(\delta -{x_1})^2} -  \frac{I^e^2}{(\delta -{x_1^{e}})^2}\right)}-{\frac{5k}{3m}{(x_1 - x_1^e)}}-{\frac{5b}{3m}x_2} \label{eq:20}
    \end{align}
    \hfill \break
    Apply Taylor's Theorem to Equation \eqref{eq:20}:
    \begin{align}
        g(I, x_1) \approx g(I^e, x_1^e) + \frac{\partial g}{\partial I_{I^e, x_1^e}}\cdot (I - I^e) + \frac{\partial g}{\partial x_{I^e, x_1^e}}\cdot (x_1 - x_1^e) \label{eq:21}
    \end{align}
    \begin{align}
        g(I, x_1) = \frac{I^2}{(\delta - x_1)^2} \label{eq:22}\\
        \frac{\partial g}{\partial I} = \frac{2I}{(\delta -{x_1})^2}\label{eq:23} \\
        \frac{\partial g}{\partial x_1} = \frac{2I^2}{(\delta -{x_1})^3} \label{eq:24}
    \end{align}
    Sub Equations \eqref{eq:22},\eqref{eq:23} and \eqref{eq:24} into \eqref{eq:21}:
    \begin{align}
         \frac{I^2}{(\delta - x_1)^2} = \frac{I^e^2}{(\delta - x_1^e)^2} + \frac{2I^e}{(\delta -{x_1^e})^2}\cdot (I - I^e) + \frac{2I^e^2}{(\delta -{x_1^e})^3}\cdot (x_1 - x_1^e) \nonumber \\
         \frac{I^2}{(\delta - x_1)^2} - \frac{I^e^2}{(\delta - x_1^e)^2} = \frac{2I^e}{(\delta -{x_1^e})^2}\cdot (I - I^e) + \frac{2I^e^2}{(\delta -{x_1^e})^3}\cdot (x_1 - x_1^e)  \label{eq:25}
    \end{align}
    Sub Equation \eqref{eq:25} into Equation \eqref{eq:20}:
    \begin{equation}
         \dot{\bar{x_2}} = \frac{5c}{3m}\left( \frac{2I^e}{(\delta -{x_1^e})^2}\cdot (I - I^e) + \frac{2I^e^2}{(\delta -{x_1^e})^3}\cdot (x_1 - x_1^e)\right) - \frac{5k}{3m}(x_1 - x_1^e) - - \frac{5b}{3m}(x_2) \label{eq:26}
    \end{equation}
    Introduce deviation variables:
    \begin{align}
         \bar{I} &= I - I^e \nonumber\\
         \bar{x_1} &= x_1 - x_1^e \nonumber\\
         \bar{x_2} &= x_2 - x_2^e = x_2 - 0 = x_2 \nonumber
    \end{align}
    to Equation \eqref{eq:26}:
    \begin{align}
         \dot{\bar{x_2}} = \frac{5c}{3m}\left( \frac{2I^e}{(\delta -{x_1^e})^2}\cdot \bar{I} + \frac{2I^e^2}{(\delta -{x_1^e})^3}\cdot \bar{x_1}\right) - \frac{5k}{3m}(\bar{x_1}) - \frac{5b}{3m}(\bar{x_2}) \nonumber \\
         \dot{\bar{x_2}} =\frac{5c2I^e}{(3m\delta -{x_1^e})^2}\cdot \bar{I} + \frac{10cI^e^2}{3m(\delta -{x_1^e})^3}\cdot \bar{x_1} - \frac{5k}{3m}(\bar{x_1}) - \frac{5b}{3m}(\bar{x_2}) \nonumber \\
         \dot{\bar{x_2}} =\frac{5c2I^e}{(3m\delta -{x_1^e})^2}\cdot \bar{I} + \left(\frac{10cI^e^2}{3m(\delta -{x_1^e})^3} - \frac{5k}{3m}\right)(\bar{x_1}) - \frac{5b}{3m}(\bar{x_2}) \label{eq:27} 
    \end{align}
    For Equation \eqref{eq:27}, let :
    \begin{equation}
         a =\frac{5c2I^e}{(3m\delta -{x_1^e})^2}, b = \left(\frac{10cI^e^2}{3m(\delta -{x_1^e})^3} - \frac{5k}{3m}\right) c = \frac{5b}{3m} \nonumber
    \end{equation}
    Subtract by parts \eqref{eq:17} and \eqref{eq:19} :
    \begin{align}
        {\dot{I}} = \frac{V - {I_1}R}{\left(L_{0} + L_{1}\exp{- \alpha y}\right)}\nonumber\\ 
        \text{--- }  0 = \frac{V^e - {I_1^e}R}{\left(L_{0} + L_{1}\exp{- \alpha (d - x)}\right)} \nonumber \\
        \rule{6cm}{1pt} \nonumber \\
        {\dot{\bar{I}}} = \frac{V - V^e - {I_1}R- {I_1^e}R}{\left(L_{0} + L_{1}\exp{- \alpha y}\right)}\label{eq:28}
    \end{align}
    Introduce deviation variables,
    \begin{align}
        \bar{V} = V - V^e \nonumber \\
        \bar{I} = I_1 - I_1^e \nonumber
    \end{align}
    to Equation \eqref{eq:28}:
    \begin{equation}\label{eq:29}
        \dot{\bar{I}} = \frac{\bar{V} - \bar{I_1}R}{\left(L_{0} + L_{1}\exp{- \alpha y}\right)}
    \end{equation}
    \hfill \break \\
    Let $f = {L_{0} + L_{1}\exp{(- \alpha y)}}$ for Equation \eqref{eq:29}\\
    \hfill \break \\
    The Linearised system equations are: \\
    \begin{align}
        \dot{\bar{x}} &= \bar{x_2}\label{eq:30} \\
        \dot{\bar{x_2}} &= a\bar{I} + b\bar{x_1} -c\bar{x_2}\label{eq:31} \\
        \dot{\bar{I}} &= \frac{1}{f}(\bar{V} - \bar{I}R)\label{eq:32}
    \end{align}